src/tls/experiments/TLS.Store.fst
@@ -1,0 +1,128 @@
+module TLS.Store
+
+module B = LowStar.Buffer
+
+module AE = Crypto.AE
+
+module HS = FStar.HyperStack
+module HST = FStar.HyperStack.ST
+
+let store_regions : (l:list substore{List.Tot.length l == 4 /\ Mem.r_pairwise_disjoint l})
+  = Mem.r_disjoint_alloc _ 4
+
+module HS = FStar.HyperStack
+
+#push-options "--z3rlimit 40 --max_fuel 4  --max_ifuel 0"
+
+val store_regions_disjoint: i:nat{i < 4} -> j:nat{j < 4} -> Lemma
+  (requires i <> j)
+  (ensures  (List.Tot.index store_regions i) `HS.disjoint` (List.Tot.index store_regions j))
+  [SMTPat (List.Tot.index store_regions i); SMTPat (List.Tot.index store_regions j)]
+
+let store_regions_disjoint i j = ()
+
+#pop-options
+
+let tls_store_server_cookie_region = List.Tot.index store_regions 0
+let tls_store_server_ticket_region = List.Tot.index store_regions 1
+
+let loc_store_regions_disjoint = ()
+
+assume val server_cookie_phi : AE.plain_pred 
+
+let server_cookie_key :
+  (server_cookie_key: B.pointer (option (a: alg & (st: AE.state a server_cookie_phi { B.loc_includes (loc_store_server_cookie_region ()) (AE.footprint st) }))) {
+    B.recallable server_cookie_key /\
+    B.frameOf server_cookie_key == tls_store_server_cookie_region
+  }) = B.gcmalloc tls_store_server_cookie_region None 1ul
+
+assume val server_ticket_phi : AE.plain_pred 
+
+let server_ticket_key :
+  (server_ticket_key: B.pointer (option (a: alg & (st: AE.state a server_ticket_phi { B.loc_includes (loc_store_server_ticket_region ()) (AE.footprint st) }))) {
+    B.recallable server_ticket_key /\
+    B.frameOf server_ticket_key == tls_store_server_ticket_region
+  }) = B.gcmalloc tls_store_server_ticket_region None 1ul
+
+unfold
+let inv' (h: HS.mem) : Tot Type0 =
+  B.live h server_cookie_key /\
+  begin match B.deref h server_cookie_key with
+  | None -> True
+  | Some (| a, st |) ->
+    B.loc_disjoint (AE.footprint st) (B.loc_buffer server_cookie_key) /\
+    AE.invariant h st
+  end /\
+  B.live h server_ticket_key /\
+  begin match B.deref h server_ticket_key with
+  | None -> True
+  | Some (| a, st |) ->
+    B.loc_disjoint (AE.footprint st) (B.loc_buffer server_ticket_key) /\
+    AE.invariant h st
+  end
+
+let inv = inv'
+
+let frame h l h' =
+  assert (Mem.loc_store_region () `B.loc_includes` B.loc_buffer server_cookie_key);
+  assert (Mem.loc_store_region () `B.loc_includes` B.loc_buffer server_ticket_key); 
+  assert (B.live h' server_cookie_key);
+  begin match B.deref h server_cookie_key with
+  | None -> ()
+  | Some (| a, st |) ->
+    assert (Mem.loc_store_region () `B.loc_includes` AE.footprint st);
+    AE.frame_invariant h st l h'
+  end;
+  assert (B.live h' server_ticket_key);
+  begin match B.deref h server_ticket_key with
+  | None -> ()
+  | Some (| a, st |) ->
+    assert (Mem.loc_store_region () `B.loc_includes` AE.footprint st);
+    AE.frame_invariant h st l h'
+  end
+
+let reset _ =
+  B.recall server_cookie_key;
+  B.recall server_ticket_key;
+  B.upd server_cookie_key 0ul None;
+  B.upd server_ticket_key 0ul None;
+  Success
+
+#push-options "--z3rlimit 16"
+
+let set_key u a key =
+  let h = HST.get () in
+  match u with
+  | ServerCookie ->
+    // TODO: free the extant one, if any; requires key to be disjoint from region
+    begin match AE.coerce tls_store_server_cookie_region a key server_cookie_phi with
+    | None -> UnsupportedAlgorithm // TODO: refine error codes
+    | Some st ->
+      let h1 = HST.get () in
+      B.upd server_cookie_key 0ul (Some (| a, st |));
+      let h' = HST.get () in
+      AE.frame_invariant h1 st (B.loc_buffer server_cookie_key) h';
+      let f () : Lemma (inv' h') =
+        begin match B.deref h server_ticket_key with
+        | None -> ()
+        | Some (| a', st' |) ->
+          AE.frame_invariant h st' (B.loc_buffer server_cookie_key) h'
+        end;
+        assert (inv' h')        
+      in
+      f ();
+      Success
+    end
+  | _ -> Success
+
+#pop-options
+
+let encrypt u plain plain_len cipher =
+  Success
+
+let decrypt u plain plain_len cipher =
+  Success
+
+(*
+let server_cookie_key :
+  (server_cookie_key: B.pointer (option (a: alg & AE.state a server_cookie_phi)) { B.frameOf server_cookie_key == store_region }) = B.gcmalloc store_region None 1ul
